gcd from class

gcd.dfy
@@ -1,9 +1,57 @@
-function gcd(m: nat, n: nat): nat
+function gcd(m: nat, n: nat) : nat
+  requires m >= 1;
+  requires n >= 1;
 {
-  if (n==m) then n
-  else if (m>n) then gcd(m-n, n)
-  else gcd(m, n-m)
+  if (m == n) then m
+  else if (m < n) then gcd(m, n-m)
+  else gcd(m-n, n)
 }
+
+lemma gcd_lemma(m: nat, n: nat)
+  requires m >= 1 && n >= 1;
+  ensures gcd(m,n) == gcd(n,m);
+{
+}
+/*
+ * Implement a method to compute
+ * greatest common divisor of two numbers m and n.
+ *
+ * A number r is a divisor of a number m iff m == r * k for some number k.
+ *
+ * If r is a divisor of m and n and m is greater than n,
+*  then r is a divisor of m-n
+ */
+method GcdCal(m: nat, n: nat) returns (res: nat)
+  requires m >= 1 && n >= 1;
+  ensures res == gcd(m, n);
+{
+  var m1: nat, n1: nat := m, n;
+
+  gcd_lemma(m, n);
+  while (m1!=n1)
+    invariant m1 >= 1;
+    invariant n1 >= 1;
+    decreases m1+n1;
+    invariant gcd(m1, n1) == gcd(n, m)
+  {
+    if (m1>n1) {
+      m1 := m1-n1;
+    }
+    else {
+      n1 := n1-m1;
+    }
+ }
+ return m1;
+}
+
+
+
+
+
+
+
+
+
 
 
 
@@ -45,7 +93,14 @@ method GcdCal(m: nat, n: nat) returns (res: nat)
 
 
 
-
+/*
+   function gcd(m: nat, n: nat): nat
+{
+  if (n==m) then n
+  else if (m>n) then gcd(m-n, n)
+  else gcd(m, n-m)
+}
+*/
 
 
 
